reflect: generate the `acc` proof

codegen/codegen.ml
@@ -8,13 +8,63 @@
 open Core
 open Errors
 
+let prelude =
+  "(*\n\
+  \ * Copyright (c) Meta Platforms, Inc. and affiliates.\n\
+  \ *\n\
+  \ * This source code is licensed under the MIT license found in the\n\
+  \ * LICENSE file in the root directory of this source tree.\n\
+  \ *)\n\
+   From stdpp Require Import base strings gmap stringmap fin_maps.\n\n\
+   From iris.proofmode Require Import tactics.\n\
+   From iris.base_logic.lib Require Import iprop own wsat.\n\
+   From iris.algebra.lib Require Import gmap_view.\n\n\
+   From shack Require Import lang progdef subtype ok typing.\n\
+   From shack Require Import eval heap modality interp soundness.\n\n\
+   From shack.reflect Require Import progdef.\n\n\
+   (* Generated from test.lang *)\n\n\
+   Definition arraykey := UnionT IntT BoolT."
+
+let mk_PDC prog =
+  let names =
+    List.map
+      ~f:(fun cdef ->
+        let name = cdef.Ast.name in
+        Printf.sprintf "\"%s\" := %s" name name)
+      prog
+  in
+  let s = String.concat ~sep:"; " names in
+  [
+    "Definition pdefs0 : stringmap classDef :=";
+    Printf.sprintf "  {[ %s ]}." s;
+    "Local Instance PDC : ProgDefContext := { pdefs := pdefs0 }.";
+    "Lemma pacc_compute:\n\
+    \  Forall\n\
+    \  (uncurry (λ (c : tag) (_ : classDef), Acc (λ x y : tag, extends y x) c))\n\
+    \  (map_to_list pdefs).\n\
+     Proof.\n\
+    \  rewrite /pdefs /= /pdefs0.\n\
+    \  apply pacc_helper.\n\
+    \  vm_compute map_to_list.\n\
+    \  simpl.\n\
+    \  rewrite Forall_lookup => k c /=.\n\
+    \  by repeat (rewrite /lookup /=; step_pacc).\n\
+     Qed.";
+    "Local Instance PDA : ProgDefAcc  := { pacc := pacc pacc_compute }.";
+  ]
+
+let process prog =
+  let l = [ prelude; Pretty.program_pretty prog ] in
+  let l = l @ mk_PDC prog in
+  String.concat ~sep:"\n\n" l
+
 let process_cmd input_file output_file =
   try
     let inx = In_channel.create input_file in
     let lexbuf = Lexing.from_channel inx in
     let raw_term = Parser.prog Lexer.lexer lexbuf in
     let () = In_channel.close inx in
-    let s = Pretty.program_pretty raw_term in
+    let s = process raw_term in
     let () =
       match output_file with
       | None -> Printf.printf "%s\n" s
