theories/reflect/progdef.v
@@ -9,7 +9,7 @@ From stdpp Require Import base strings gmap stringmap fin_maps.
 From iris.proofmode Require Import tactics.
 From shack Require Import lang progdef.
 
-Section Reflect.
+Section Extends.
   (* assume a given set of class definitions *)
   Context `{PDC: ProgDefContext}.
 
@@ -33,14 +33,70 @@ Section Reflect.
       destruct (B =? B) eqn:h; first done.
       by rewrite eqb_neq in h.
   Qed.
+End Extends.
 
-  Lemma pacc_helper (P: tag → Prop) (xdefs: stringmap classDef):
-    Forall P (map fst (map_to_list xdefs)) →
-    Forall (uncurry (λ c _, P c)) (map_to_list xdefs).
-  Proof.
-    rewrite Forall_lookup => h.
+Lemma pacc_helper (P: tag → Prop) (xdefs: stringmap classDef):
+  Forall P (map fst (map_to_list xdefs)) →
+  Forall (uncurry (λ c _, P c)) (map_to_list xdefs).
+Proof.
+  rewrite Forall_lookup => h.
   rewrite Forall_lookup => k [c ?] hk /=.
   apply h with k.
   by rewrite list_lookup_fmap hk.
-  Qed.
-End Reflect.
+Qed.
+
+(* Helper tactics to deal with the `Acc` goal in progdef.v *)
+Lemma string_eqb_correct (s t: string) : (s =? t)%string ↔ s = t.
+Proof.
+  destruct String.eqb eqn:h.
+  - by apply String.eqb_eq in h as ->.
+  - apply String.eqb_neq in h.
+    by split.
+Qed.
+
+(* Do one step of Accessibility *)
+Ltac simpl_acc0 :=
+  constructor => ? /extendsb_correct;
+  rewrite /extendsb /=;
+  simpl_map => /=.
+
+(* If the previous tactic didn't solve the goal,
+ * rewrite.
+ *)
+Ltac simpl_acc1 := move/string_eqb_correct => ->.
+
+(* Gluing both tactics into an automated one *)
+Ltac simpl_acc_match :=
+  match goal with
+  | |- False → _ => done
+  | |- _ => (simpl_acc1; simpl_acc0)
+  end.
+
+Ltac simpl_acc := simpl_acc0; repeat simpl_acc_match.
+
+Ltac step_pacc :=
+  match goal with
+  | |- None = Some ?t → _ => done
+  | H : nat |- _ => destruct H; first (case => <-; simpl_acc)
+  end.
+
+Definition pacc_uncurry_def `{PDC: ProgDefContext} :=
+  Forall (uncurry (λ c _, Acc (λ x y : tag, extends y x) c))
+         (map_to_list pdefs).
+
+Lemma pacc `{PDC: ProgDefContext}:
+  pacc_uncurry_def → ∀ c, Acc (λ x y : tag, extends y x) c.
+Proof.
+  move => hacc.
+  assert (pacc_ : map_Forall (λ c _, Acc (λ x y, extends y x) c) pdefs).
+  { rewrite map_Forall_to_list /=.
+    by apply hacc.
+  }
+  move => c.
+  destruct (pdefs !! c) as [cdef | ] eqn:hcdef.
+  - move : pacc_ => /map_Forall_lookup h.
+    by eapply h.
+  - constructor => t hext; exfalso.
+    inv hext.
+    by simplify_eq.
+Qed.
